Ac_simp works (partially, since it doesn't work with duplicate removal)! Added some tests

src/verit/veritAst.ml
@@ -399,7 +399,7 @@ let process_rule (r: rule) : VeritSyntax.typ =
   | ImpsimpAST -> raise (Debug ("| process_rule: implies_simplify should be eliminated|"))
   | EqsimpAST -> raise (Debug ("| process_rule: equiv_simplify should be eliminated|"))
   | BoolsimpAST -> raise (Debug ("| process_rule: bool_simplify should be eliminated|"))
-  | AcsimpAST -> Flatten
+  | AcsimpAST -> Acsimp
   | ItesimpAST -> raise (Debug ("| process_rule: ite_simplify should be eliminated|"))
   | EqualsimpAST -> raise (Debug ("| process_rule: equal_simplify should be eliminated|"))
   | DistelimAST -> Distelim
