ACSIMP.md
@@ -1,0 +1,83 @@
+# Checker for `ac_simp`
+
+`ac_simp` is a tautological rule (a rule that takes no premises) in the Alethe proof format. It reduces arbitrary and/or chains in 2 ways:
+1. Flatten applications (ex: `a v (b v c) = a v b v c`)
+2. Remove duplicates (ex: `a ^ b ^ b = a ^ b`)
+
+The `Flatten` rule in SMTCOQ takes two formulas as input and checks that they are equivalent, in particular up to flattening. Its checker is in `Syntactic.v` (see `check_flatten_body`).
+It remains to be confirmed whether it removes duplicates.
+
+## Approach 1 (Unfeasible)
+Since `ImmFlatten` (the SmtCertif version of `Flatten`) is a premise-conclusion rule and `ac_simp` is a tautological
+rule proving equivalence `x = y`, this approach 
+tries to create a new clause that derives `x` 
+using `mkRootV` and then derive `y` from `x` using `ImmFlatten`.
+
+*Problem:* Roots are only for initial assumptions and they can't be used to insert 
+arbitrary steps into the certificate.
+
+## Approach 2 (Unfeasible)
+Given `x = y` proven by `ac_simp`, introduce two subproofs:
+```
+--assume
+x
+--ImmFlatten
+y
+
+--assume
+y
+--ImmFlatten
+x
+```
+and then process them using `process_subproof`.
+
+*Problem:* `ImmFlatten` is a premise-conclusion rule, and `process_subproof` will fail on it because it expects all rules to be tautological. For example:
+```
+Certif after process_subproof: 
+(h1, AssumeAST, (cl  ((not ((and  a (and  b c)) = (and  a b c))))), [], [])
+(x7, Equn1AST, (cl  (((and  a (and  b c)) = (and  a b c))) ((not (and  a (and  b c)))) ((not (and  a b c)))), [], [])
+(x5, AndnAST, (cl  ((and  (and  a (and  b c)) (not (and  a b c)))) ((not (and  a (and  b c)))) ((and  a b c))), [], [])
+(x9, ResoAST, (cl  ((and  (and  a (and  b c)) (not (and  a b c)))) (((and  a (and  b c)) = (and  a b c))) ((not (and  a (and  b c))))), [ x5 x7], [])
+(x8, Equn2AST, (cl  (((and  a (and  b c)) = (and  a b c))) ((and  a (and  b c))) ((and  a b c))), [], [])
+(x6, AndnAST, (cl  ((and  (and  a b c) (not (and  a (and  b c))))) ((not (and  a b c))) ((and  a (and  b c)))), [], [])
+(x10, ResoAST, (cl  ((and  (and  a b c) (not (and  a (and  b c))))) (((and  a (and  b c)) = (and  a b c))) ((and  a (and  b c)))), [ x6 x8], [])
+(t2, ResoAST, (cl  ((and  (and  a (and  b c)) (not (and  a b c)))) ((and  (and  a b c) (not (and  a (and  b c))))) (((and  a (and  b c)) = (and  a b c)))), [ x9 x10], [])
+(t3, ResoAST, (cl  ((and  (and  a (and  b c)) (not (and  a b c)))) ((and  (and  a b c) (not (and  a (and  b c)))))), [ h1 t2], [])
+(x14, AndpAST, (cl  ((not (and  (and  a b c) (not (and  a (and  b c)))))) ((and  a b c))), [], [ 0])
+(x13, ResoAST, (cl  ((and  (and  a (and  b c)) (not (and  a b c)))) ((and  a b c))), [ t3 x14], [])
+(x4, AcsimpAST, (cl  ((and  a (and  b c)))), [ x13], [])
+(x15, AndpAST, (cl  ((not (and  (and  a b c) (not (and  a (and  b c)))))) ((not (and  a (and  b c))))), [], [ 1])
+(x16, ResoAST, (cl  ((and  (and  a (and  b c)) (not (and  a b c)))) ((not (and  a (and  b c))))), [ t3 x15], [])
+(x17, ResoAST, (cl  ((and  (and  a (and  b c)) (not (and  a b c))))), [ x4 x16], [])
+(x19, AndpAST, (cl  ((not (and  (and  a (and  b c)) (not (and  a b c))))) ((and  a (and  b c)))), [], [ 0])
+(x18, ResoAST, (cl  ((and  a (and  b c)))), [ x17 x19], [])
+(x3, AcsimpAST, (cl  ((and  a b c))), [ x18], [])
+(x20, AndpAST, (cl  ((not (and  (and  a (and  b c)) (not (and  a b c))))) ((not (and  a b c)))), [], [ 1])
+(x21, ResoAST, (cl  ((not (and  a b c)))), [ x17 x20], [])
+(x22, ResoAST, (cl ), [ x3 x21], [])
+```
+Here, we expect `x13` and `x4` to represent:
+```
+and a b c
+---------------------ImmFlatten
+and a (and b c)
+```
+but instead we have:
+```
+((and  (and  a (and  b c)) (not (and  a b c)))) ((and  a b c)))
+-------------------------------------------------------------------------------ImmFlatten
+and a (and b c)
+```
+
+## Approach 3
+Add `Flatten` - the non `Imm` version of `ImmFlatten` to `SmtCertif`. Use the Coq code that already exists for
+the checker for `ImmFlatten` in SMTCoq. It should be 
+reusable. Now `ac_simp` simply reduces to `Flatten`.
+
+This works for flattening! Note that it doesn't work if the literals in the or/and are reordered, but this 
+should be okay. For example: `ac_simp` can't prove `(= (or a b c) (or (or b a) c))` but it can prove
+`(= (or a b c) (or (or a b) c))`.
+
+However, it doesn't work for duplicate removal. This needs to be added to the checker maybe. From 
+`examples/aletheTests/testrewrites/`, `acsimp.v` and `acsimp2.v` are successful tests for flattening in
+by `ac_simp` and `acsimp3.v` is a failed test showing that duplicate removal doesn't work.
